commit before refactoring

Core/TracesFacts.v
@@ -1,5 +1,6 @@
 From LHL.Util Require Import
-  Util.
+  Util
+  TransUtil.
 
 From LHL.Core Require Import
     Program
@@ -7,12 +8,16 @@ From LHL.Core Require Import
     Traces
     Eutt.
 
+(* Basic Trace Properties *)
+
 Lemma nil_IsTraceOfSpec {E} :  
     forall (spec : Spec E),
     IsTraceOfSpec nil spec.
 Proof.
     intros. exists spec.(Init). apply TransUtil.StepsNone.
 Qed.
+
+(* Step Properties *)
 
 (* Eutt *)
 
@@ -30,3 +35,24 @@ Definition euttTS {E E' : ESig}  (RR : IRel E E') :
     ThreadsSt (E := E) -> ThreadsSt (E := E') -> Prop :=
     fun ths ths' => forall (i : ThreadName), euttTS_ RR (ths i) (ths' i).
 
+Definition euttIS {A E E'} (RR : IRel E E') :
+    ThreadsSt (E := E) * A -> ThreadsSt (E := E') * A -> Prop :=
+        fun ost ost' => euttTS RR (fst ost) (fst ost').
+
+Lemma eutt_InterStep {E F} (RR : IRel E E) (spec : Spec E) (impl : Impl E F) (impl' : Impl E F): 
+    euttImpl RR impl impl' ->
+    forall i ist0 ev ist1 ist0',
+        euttIS (A := spec.(State)) RR ist0 ist0' ->
+        InterStep (impl := impl) i ist0 ev ist1 ->
+        exists ist1' ev',
+            (ev' = ev \/ ev' = (i, Silent)) /\
+            InterStep (impl := impl') i ist0' ev' ist1'.
+
+Lemma euttTS_isPathOf {E F} (spec : Spec E) : 
+    forall (impl : Impl E F) (impl' : Impl E F),
+    forall t thst0 thst1 thst0', 
+        euttOS ieq thst0 thst0' ->
+        IsPathOf thst0 t thst1 (Steps (overObj (spec :> impl)).(Step)) ->
+        exists thst1',  
+            IsPathOf thst0' t thst1' (Steps (overObj (spec :> impl')).(Step)).
+Admitted.
