Core/Program.v
@@ -1,11 +1,6 @@
 Definition ESig : Type := Type -> Type.
 
-Inductive Sum {E F : ESig} : ESig :=
-| InL {A} (x : E A) : Sum A
-| InR {A} (x : F A) : Sum A.
-Arguments Sum : clear implicits.
-
-Notation "E |+| F" := (Sum E F) (at level 41, right associativity).
+Definition Sum EL ER (Ret : Type) := sum (EL Ret) (ER Ret).
 
 CoInductive Prog {E : ESig} {Ret : Type} : Type :=
 | Bind {A} : E A -> (A -> Prog) -> Prog
