Core/Tensor.v
@@ -1,0 +1,25 @@
+From LHL.Core Require Import
+  Program
+  Specs.
+
+Section Tensor.
+  Context {EL ER}
+          (specL : Spec EL)
+          (specR : Spec ER).
+
+  Definition StepTensor st (ev : ThreadEvent (Sum EL ER)) st' :=
+    match ev with
+      | CallEv m => inl ev' => specL.(EvalInstruction) instr' (fst st) a (fst st') /\ (snd st = snd st')
+      | CallEv n => inr instr' => specR.(EvalInstruction) instr' (snd st) a (snd st') /\ (fst st = fst st')
+    end.
+
+  Definition pairSpec : Spec PairInstruction :=
+    {|
+      State := prod specL.(State) specR.(State);
+      EvalInstruction := EvalPairInstruction;
+      initialState := (specL.(initialState), specR.(initialState))
+    |}.
+
+End Pair.
+
+Arguments PairInstruction : clear implicits.
